Hashmap/DHashMap/ForUpstream.lean
@@ -4,7 +4,7 @@ Copyright (c) 2024 Lean FRO, LLC. All rights reserved.
 Released under Apache 2.0 license as described in the file LICENSE.
 Authors: Markus Himmel
 -/
-import Std.Data.List.Perm
+import Batteries.Data.List.Perm
 
 open List
 
