lakefile.lean
@@ -11,4 +11,4 @@ lean_lib «Hashmap» where
 lean_exe «hashmap» where
   root := `Main
 
-require std from git "https://github.com/leanprover/std4" @ "48643957cb394f0740a292b14954747c96bcd00e"
+require batteries from git "https://github.com/leanprover-community/batteries" @ "main"
